\documentclass{article}

\usepackage{amsmath}
\usepackage{siunitx}
\usepackage{graphicx}

\newcommand{\del}[2]{\frac{\partial #1}{\partial #2}}  % Partial derivative
\newcommand{\ddel}[2]{\frac{\partial^2 #1}{\partial #2^2}}  % Partial second derivative
\newcommand{\deriv}[2]{\frac{\mathrm{d} #1}{\mathrm{d} #2}}  % Derivative
\newcommand{\dderiv}[2]{\frac{\mathrm{d}^2 #1}{\mathrm{d} #2^2}}  % Second derivative

\begin{document}
\noindent\textbf{Task 2.2}\\
Let $t = t' t_0$ and $x=x' x_0$.
Setting $t_0 = L$ we getjj
$$
-\frac{\hbar^2}{2mL^2} \ddel{\Psi}{x'} = \frac{i\hbar}{t_0} \del{\Psi}{t'},
$$
and we see that setting $t_0 = \frac{2mL^2}{\hbar}$ gives us
$$
-\ddel{\Psi}{x'} = i \del{\Psi}{t'}.
$$


\noindent\textbf{Task 2.3}\\
(2.7) therefor gives
$$
-\ddel{\psi_n}{x'} = \frac{E_n 2mL^2}{\hbar^2} \psi_n
$$
or
$$
\ddel{\psi_n}{x'} = \lambda_n \psi_n,
$$
where we defined
$$
\lambda_n = \frac{2mL^2}{\hbar^2} E_n.
$$
\end{document}
